fold protocol-following logic into Modules.v and Example2.v
not fully hooked up into the end-to-end stack yet, though

src/Spec/Example2.v
@@ -188,6 +188,67 @@ Module CounterAPI <: Layer.
 End CounterAPI.
 
 
+(** Locking discipline *)
+
+Module LockingRule <: ProcRule LockAPI.
+
+  Definition follows_protocol_op `(op : LockAPI.opT T) (tid : nat)
+                                  (old_owner : bool) (new_owner : bool) :=
+    match op with
+    | Acquire => old_owner = false /\ new_owner = true
+    | Release => old_owner = true /\ new_owner = false
+    | Read => old_owner = true /\ new_owner = true
+    | Write _ => old_owner = true /\ new_owner = true
+    end.
+
+  Definition lock_match s tid :=
+    match Lock s with
+    | Some tid' =>
+      if tid' == tid then true else false
+    | None => false
+    end.
+
+  Inductive follows_protocol_proc (tid : nat) (old_owner : bool) (new_owner : bool) :
+    forall T (p : proc LockAPI.opT T), Prop :=
+  | FollowsProtocolProcOp :
+    forall T (op : LockAPI.opT T),
+    follows_protocol_op op tid old_owner new_owner ->
+    follows_protocol_proc tid old_owner new_owner (Op op)
+  | FollowsProtocolProcBind :
+    forall T1 T2 (p1 : proc _ T1) (p2 : T1 -> proc _ T2) mid_owner,
+    follows_protocol_proc tid old_owner mid_owner p1 ->
+    (forall x, follows_protocol_proc tid mid_owner new_owner (p2 x)) ->
+    follows_protocol_proc tid old_owner new_owner (Bind p1 p2)
+  | FollowsProtocolProcUntil :
+    forall T (p : proc _ T) c,
+    old_owner = new_owner ->
+    follows_protocol_proc tid old_owner new_owner p ->
+    follows_protocol_proc tid old_owner new_owner (Until c p)
+  | FollowsProtocolProcAtomic :
+    forall T (p : proc _ T),
+    follows_protocol_proc tid old_owner new_owner p ->
+    follows_protocol_proc tid old_owner new_owner (Atomic p)
+  | FollowsProtocolProcLog :
+    forall T (v : T),
+    old_owner = new_owner ->
+    follows_protocol_proc tid old_owner new_owner (Log v)
+  | FollowsProtocolProcRet :
+    forall T (v : T),
+    old_owner = new_owner ->
+    follows_protocol_proc tid old_owner new_owner (Ret v).
+
+  Definition follows_protocol_s (ts : @threads_state LockAPI.opT) (s : LockAPI.State) :=
+    forall tid T (p : proc _ T),
+      ts [[ tid ]] = Proc p ->
+      exists b,
+        follows_protocol_proc tid (lock_match s tid) b p.
+
+  Definition follows_protocol ts :=
+    forall s, follows_protocol_s ts s.
+
+End LockingRule.
+
+
 (** Using locks to get atomicity. *)
 
 Module LockingCounter <: LayerImpl LockAPI LockedCounterAPI.
@@ -351,6 +412,17 @@ Module LockingCounter <: LayerImpl LockAPI LockedCounterAPI.
     eapply all_traces_match; eauto.
     eapply Compile.compile_ts_ok; eauto.
   Qed.
+
+(*
+  Theorem compile_ts_follows_protocol :
+    forall ts,
+      no_atomics_ts ts ->
+      LockingRule.follows_protocol (compile_ts ts).
+  Proof.
+    unfold LockingRule.follows_protocol; intros.
+    induction ts; intros.
+    - unfold LockingRule.follows_protocol_s.
+*)
 
 End LockingCounter.
 
@@ -535,6 +607,292 @@ Module LockImpl <: LayerImpl TASLockAPI RawLockAPI.
 End LockImpl.
 
 
+(** Locking discipline *)
+
+Module LockProtocol <: LayerImplRequiresRule RawLockAPI LockAPI LockingRule.
+
+  Import LockingRule.
+
+  Definition absR (s1 : RawLockAPI.State) (s2 : LockAPI.State) :=
+    s1 = s2.
+
+  Ltac step_inv :=
+    match goal with
+    | H : RawLockAPI.step _ _ _ _ _ |- _ =>
+      inversion H; clear H; subst; repeat sigT_eq
+    | H : LockAPI.step _ _ _ _ _ |- _ =>
+      inversion H; clear H; subst; repeat sigT_eq
+    end.
+
+  Theorem follows_protocol_step : forall `(op : LockAPI.opT T) tid s v s' b,
+    RawLockAPI.step op tid s v s' ->
+    follows_protocol_op op tid (lock_match s tid) b ->
+    LockAPI.step op tid s v s'.
+  Proof.
+    intros.
+    destruct s.
+    step_inv; unfold lock_match in *; simpl in *.
+    - eauto.
+    - destruct Lock0; [ destruct (n == tid) | ]; subst; simpl in *;
+        intuition eauto; congruence.
+    - destruct Lock0; [ destruct (n == tid) | ]; subst; simpl in *;
+        intuition eauto; congruence.
+    - destruct Lock0; [ destruct (n == tid) | ]; subst; simpl in *;
+        intuition eauto; congruence.
+  Qed.
+
+  Hint Resolve follows_protocol_step.
+  Hint Constructors follows_protocol_proc.
+
+
+  Lemma follows_protocol_op_owner : forall `(op : RawLockAPI.opT T) tid s v s' b,
+    RawLockAPI.step op tid s v s' ->
+    follows_protocol_op op tid (lock_match s tid) b ->
+    b = lock_match s' tid.
+  Proof.
+    intros; step_inv; unfold lock_match in *; simpl in *;
+      intuition try congruence.
+    destruct (tid == tid); congruence.
+  Qed.
+
+  Theorem follows_protocol_atomic_owner :
+    forall `(p : proc RawLockAPI.opT T) tid s0 r s1 evs b,
+    atomic_exec RawLockAPI.step p tid s0 r s1 evs ->
+    follows_protocol_proc tid (lock_match s0 tid) b p ->
+    b = lock_match s1 tid.
+  Proof.
+    intros.
+    generalize dependent b.
+    induction H; simpl in *; intros; eauto;
+      match goal with
+      | H : follows_protocol_proc _ _ _ _ |- _ =>
+        inversion H; clear H; repeat sigT_eq; subst
+      end; eauto.
+    - repeat deex.
+      eapply IHatomic_exec1 in H5; subst.
+      specialize (H7 v1); eauto.
+    - eapply follows_protocol_op_owner; eauto.
+    - erewrite <- IHatomic_exec. reflexivity.
+      econstructor; eauto; intros.
+      destruct (Bool.bool_dec (c x)).
+      constructor; eauto.
+      constructor; eauto.
+  Qed.
+
+  Theorem follows_protocol_atomic : forall `(p : proc RawLockAPI.opT T) tid s v s' evs b,
+    atomic_exec RawLockAPI.step p tid s v s' evs ->
+    follows_protocol_proc tid (lock_match s tid) b p ->
+    atomic_exec LockAPI.step p tid s v s' evs.
+  Proof.
+    intros.
+    erewrite follows_protocol_atomic_owner with (b0 := b) in H0; eauto.
+    induction H; intros; eauto;
+      match goal with
+      | H : follows_protocol_proc _ _ _ _ |- _ =>
+        inversion H; clear H; repeat sigT_eq; subst
+      end; eauto.
+
+    eapply follows_protocol_atomic_owner in H5 as H5'; eauto; subst.
+    eauto.
+
+    constructor.
+    eapply IHatomic_exec.
+    econstructor; eauto; intros.
+    destruct (Bool.bool_dec (c x)).
+    constructor; eauto.
+    constructor; eauto.
+    congruence.
+  Qed.
+
+  Hint Resolve follows_protocol_atomic.
+
+
+  Lemma follows_protocol_exec_tid :
+    forall ts tid `(p : proc _ T) s s' result evs,
+      follows_protocol_s ts s ->
+      ts [[ tid ]] = Proc p ->
+      exec_tid RawLockAPI.step tid s p s' result evs ->
+      exec_tid LockAPI.step tid s p s' result evs.
+  Proof.
+    intros.
+    specialize (H tid _ p); intuition idtac; deex.
+    generalize dependent ts.
+    generalize dependent b.
+    induction H1; simpl in *; intros; eauto;
+      match goal with
+      | H : follows_protocol_proc _ _ _ _ |- _ =>
+        inversion H; clear H; repeat sigT_eq; subst
+      end; eauto.
+
+    constructor.
+    eapply IHexec_tid.
+    eauto.
+    rewrite thread_upd_eq with (ts := ts). reflexivity.
+  Qed.
+
+
+  Lemma lock_match_op_ne : forall `(op : RawLockAPI.opT T) tid tid' s s' r b,
+    RawLockAPI.step op tid s r s' ->
+    follows_protocol_op op tid (lock_match s tid) b ->
+    tid <> tid' ->
+    lock_match s tid' = lock_match s' tid'.
+  Proof.
+    intros.
+    step_inv; unfold lock_match in *; simpl in *.
+    destruct (tid == tid'); congruence.
+    all: destruct l; eauto.
+    destruct (n == tid); destruct (n == tid'); subst; intuition congruence.
+  Qed.
+
+  Hint Resolve lock_match_op_ne.
+
+
+  Lemma lock_match_atomic_ne : forall `(p : proc RawLockAPI.opT T) tid tid' s s' r evs b,
+    atomic_exec RawLockAPI.step p tid s r s' evs ->
+    follows_protocol_proc tid (lock_match s tid) b p ->
+    tid <> tid' ->
+    lock_match s tid' = lock_match s' tid'.
+  Proof.
+    intros.
+    generalize dependent b.
+    induction H; simpl in *; intros; eauto;
+      match goal with
+      | H : follows_protocol_proc _ _ _ _ |- _ =>
+        inversion H; clear H; repeat sigT_eq; subst
+      end; eauto.
+
+    intuition idtac.
+    eapply follows_protocol_atomic_owner in H6 as H6'; eauto; subst.
+    erewrite H2; eauto.
+
+    intuition idtac.
+    eapply H0.
+    econstructor; eauto; intros.
+    destruct (Bool.bool_dec (c x)).
+    constructor; eauto.
+    constructor; eauto.
+  Qed.
+
+  Hint Resolve lock_match_atomic_ne.
+
+
+  Lemma lock_match_exec_tid_ne : forall `(p : proc RawLockAPI.opT T) tid tid' s s' r evs b,
+    exec_tid RawLockAPI.step tid s p s' r evs ->
+    follows_protocol_proc tid (lock_match s tid) b p ->
+    tid <> tid' ->
+    lock_match s tid' = lock_match s' tid'.
+  Proof.
+    intros.
+    generalize dependent b.
+    induction H; simpl in *; intros; eauto;
+      match goal with
+      | H : follows_protocol_proc _ _ _ _ |- _ =>
+        inversion H; clear H; repeat sigT_eq; subst
+      end; eauto.
+  Qed.
+
+  Lemma follows_protocol_proc_exec_tid :
+    forall `(p : proc RawLockAPI.opT T) tid s s' p' evs b,
+    follows_protocol_proc tid (lock_match s tid) b p ->
+    exec_tid RawLockAPI.step tid s p s' (inr p') evs ->
+    follows_protocol_proc tid (lock_match s' tid) b p'.
+  Proof.
+    intros.
+    remember (inr p').
+    generalize dependent p'.
+    generalize dependent b.
+    induction H0; intros; simpl in *; try congruence.
+
+    match goal with
+    | H : follows_protocol_proc _ _ _ _ |- _ =>
+      inversion H; clear H; repeat sigT_eq; subst
+    end; eauto.
+
+    inversion Heqs0; clear Heqs0; subst.
+    destruct result.
+    - inversion H0; repeat sigT_eq; simpl in *; subst;
+                    repeat sigT_eq; simpl in *; subst; eauto;
+        match goal with
+        | H : follows_protocol_proc _ _ _ _ |- _ =>
+          inversion H; clear H; repeat sigT_eq; subst
+        end; eauto.
+      eapply follows_protocol_op_owner in H2; eauto; subst; eauto.
+      eapply follows_protocol_atomic_owner in H2; eauto; subst; eauto.
+    - specialize (IHexec_tid _ H4 _ eq_refl).
+      simpl. eauto.
+    - inversion Heqs0; clear Heqs0; subst.
+      inversion H; clear H; repeat sigT_eq; subst.
+      econstructor; eauto; intros.
+      destruct (Bool.bool_dec (c x)).
+      constructor; eauto.
+      constructor; eauto.
+  Qed.
+
+  Lemma follows_protocol_exec_tid_upd :
+    forall ts tid `(p : proc _ T) s s' result evs,
+      follows_protocol_s ts s ->
+      ts [[ tid ]] = Proc p ->
+      exec_tid RawLockAPI.step tid s p s' result evs ->
+      follows_protocol_s ts [[ tid := match result with
+                                      | inl _ => NoProc
+                                      | inr p' => Proc p'
+                                      end ]] s'.
+  Proof.
+    unfold follows_protocol_s; intros.
+    destruct (tid == tid0); subst.
+    - autorewrite with t in *.
+      destruct result; try congruence.
+      repeat maybe_proc_inv.
+      specialize (H _ _ _ H0); deex.
+
+      eexists.
+      eapply follows_protocol_proc_exec_tid; eauto.
+
+    - autorewrite with t in *.
+      specialize (H _ _ _ H2) as Ha; deex.
+      specialize (H _ _ _ H0) as Hb; deex.
+      erewrite <- lock_match_exec_tid_ne; eauto.
+  Qed.
+
+  Definition compile_ts (ts : @threads_state LockAPI.opT) := ts.
+
+  Theorem compile_ts_no_atomics :
+    forall ts,
+      no_atomics_ts ts ->
+      no_atomics_ts (compile_ts ts).
+  Proof.
+    unfold compile_ts; eauto.
+  Qed.
+
+  Theorem compile_traces_match :
+    forall ts,
+      follows_protocol ts ->
+      no_atomics_ts ts ->
+      traces_match_abs absR RawLockAPI.step LockAPI.step (compile_ts ts) ts.
+  Proof.
+    unfold compile_ts, follows_protocol, absR.
+    unfold traces_match_abs; intros; subst.
+    clear H0.
+    destruct H1.
+    specialize (H sm).
+    induction H0; eauto.
+    specialize (H tid _ p) as Htid.
+    intuition idtac; repeat deex.
+
+    edestruct IHexec.
+      eapply follows_protocol_exec_tid_upd; eauto.
+
+    eexists; intuition idtac.
+    eapply ExecPrefixOne.
+      eauto.
+      eapply follows_protocol_exec_tid; eauto.
+      eauto.
+    eauto.
+  Qed.
+
+End LockProtocol.
+
+
 (** Linking *)
 
 (* End-to-end stack:
@@ -544,7 +902,7 @@ End LockImpl.
   TASLockAPI
     [ LockImpl ]
   RawLockAPI
-    [ ?? ]
+    [ LockProtocol ]
   LockAPI
     [ LockingCounter ]
   LockedCounterAPI
