src/Spec/Modules.v
@@ -40,6 +40,13 @@ Module Type Layer.
 End Layer.
 
 
+Module Type ProcRule (l : Layer).
+
+  Axiom follows_protocol : @threads_state l.opT -> Prop.
+
+End ProcRule.
+
+
 Module Type LayerImpl (l1 : Layer) (l2 : Layer).
 
   Axiom absR : l1.State -> l2.State -> Prop.
@@ -56,10 +63,48 @@ Module Type LayerImpl (l1 : Layer) (l2 : Layer).
 End LayerImpl.
 
 
+Module Type LayerImplRequiresRule (l1 : Layer) (l2 : Layer) (r : ProcRule l2).
+
+  Axiom absR : l1.State -> l2.State -> Prop.
+  Axiom compile_ts : @threads_state l2.opT -> @threads_state l1.opT.
+  Axiom compile_ts_no_atomics :
+    forall ts,
+      no_atomics_ts ts ->
+      no_atomics_ts (compile_ts ts).
+  Axiom compile_traces_match :
+    forall ts,
+      r.follows_protocol ts ->
+      no_atomics_ts ts ->
+      traces_match_abs absR l1.step l2.step (compile_ts ts) ts.
+
+End LayerImplRequiresRule.
+
+
+Module Type LayerImplFollowsRule (l1 : Layer) (l2 : Layer) (r : ProcRule l1).
+
+  Axiom absR : l1.State -> l2.State -> Prop.
+  Axiom compile_ts : @threads_state l2.opT -> @threads_state l1.opT.
+  Axiom compile_ts_no_atomics :
+    forall ts,
+      no_atomics_ts ts ->
+      no_atomics_ts (compile_ts ts).
+  Axiom compile_ts_follows_protocol :
+    forall ts,
+      no_atomics_ts ts ->
+      r.follows_protocol (compile_ts ts).
+  Axiom compile_traces_match :
+    forall ts,
+      no_atomics_ts ts ->
+      traces_match_abs absR l1.step l2.step (compile_ts ts) ts.
+
+End LayerImplFollowsRule.
+
+
 (** General layer transformers. *)
 
-Module Link (a : Layer) (b : Layer) (c : Layer)
-            (x : LayerImpl a b) (y : LayerImpl b c) <: LayerImpl a c.
+Module Link
+  (a : Layer) (b : Layer) (c : Layer)
+  (x : LayerImpl a b) (y : LayerImpl b c) <: LayerImpl a c.
 
   Definition absR (s1 : a.State) (s3 : c.State) :=
     exists s2, x.absR s1 s2 /\ y.absR s2 s3.
@@ -93,3 +138,42 @@ Module Link (a : Layer) (b : Layer) (c : Layer)
   Qed.
 
 End Link.
+
+
+Module LinkWithRule
+  (a : Layer) (b : Layer) (c : Layer) (r : ProcRule b)
+  (x : LayerImplRequiresRule a b r) (y : LayerImplFollowsRule b c r) <: LayerImpl a c.
+
+  Definition absR (s1 : a.State) (s3 : c.State) :=
+    exists s2, x.absR s1 s2 /\ y.absR s2 s3.
+
+  Definition compile_ts ts :=
+    x.compile_ts (y.compile_ts ts).
+
+  Theorem compile_ts_no_atomics :
+    forall ts,
+      no_atomics_ts ts ->
+      no_atomics_ts (compile_ts ts).
+  Proof.
+    intros.
+    eapply x.compile_ts_no_atomics.
+    eapply y.compile_ts_no_atomics.
+    eauto.
+  Qed.
+
+  Theorem compile_traces_match :
+    forall ts,
+      no_atomics_ts ts ->
+      traces_match_abs absR a.step c.step (compile_ts ts) ts.
+  Proof.
+    unfold traces_match_abs; intros.
+    inversion H1; clear H1; intuition idtac.
+    edestruct x.compile_traces_match; intuition eauto.
+      eapply y.compile_ts_follows_protocol; eauto.
+      eapply y.compile_ts_no_atomics; eauto.
+    edestruct y.compile_traces_match; intuition eauto.
+    eexists; intuition eauto.
+    etransitivity; eauto.
+  Qed.
+
+End LinkWithRule.
